cedar-lean/Cedar/Thm.lean
@@ -18,4 +18,5 @@ import Cedar.Thm.Data
 import Cedar.Thm.Authorization
 import Cedar.Thm.Slicing
 import Cedar.Thm.Typechecking
+import Cedar.Thm.Entities
 import Cedar.Thm.Validation
