cedar-lean/Cedar/Thm/Entities.lean
@@ -1,0 +1,37 @@
+
+import Batteries.Data.List
+import Cedar.Spec.Entities
+import Cedar.Data.Map
+namespace Cedar.Thm
+
+open Cedar.Data
+open Cedar.Spec
+
+
+def subslice (e₁ e₂ : Entities) : Prop :=
+  ∀ (euid : EntityUID) (edata),
+    e₁.find? euid = some edata →
+    e₁.find? euid = e₂.find? euid
+
+theorem subslice_refl (e : Entities) :
+  subslice e e
+  := by
+  simp [subslice]
+
+theorem subslice_trans (e₁ e₂ e₃ : Entities)
+  (h₁ : subslice e₁ e₂)
+  (h₂ : subslice e₂ e₃) :
+  subslice e₁ e₃
+  := by
+  simp [subslice] at *
+  intros euid edata h
+  have step₁ : Map.find? e₁ euid = Map.find? e₂ euid := by
+    apply h₁
+    apply h
+  have step₂ : Map.find? e₂ euid = Map.find? e₃ euid := by
+    apply h₂
+    rw [← step₁]
+    apply h
+  simp [step₁, step₂]
+
+end Cedar.Thm
